new setoid rewrite + plugin fixes + proofs

theories/Lambda/AutoSetoidRewrite2.v
@@ -27,6 +27,7 @@ Section setoid.
   Context {RSymOk_func : RSymOk RSym_func}.
   Context {Typ0_Prop : Typ0 _ Prop}.
   Context {RelDec_eq_typ : RelDec (@eq typ)}.
+  Context {RelDec_Correct_eq_typ : RelDec_Correct RelDec_eq_typ}.
   Context {RelDec_eq_func : RelDec (@eq func)}.
 
   Let tyArr : typ -> typ -> typ := @typ2 _ _ _ _.
@@ -212,31 +213,397 @@ Section setoid.
     Qed.
   End setoid_rewrite.
 
-  Section bottom_up.
+  Section top_bottom.
     Context (reflexive transitive : R -> bool)
             (rw : expr typ func -> R -> option (expr typ func))
-            (respectful : expr typ func -> list (expr typ func) -> R -> option (list R)).
+            (respectful : expr typ func -> R -> option (list R)).
+
+    Hypothesis reflexiveOk
+    : forall r t rD, reflexive r = true -> RD r t = Some rD -> Reflexive rD.
+    Hypothesis transitiveOk
+    : forall r t rD, transitive r = true -> RD r t = Some rD -> Transitive rD.
+    Hypothesis rwOk
+    : forall tus tvs e e' r t eD rD,
+        rw e r = Some e' ->
+        RD r t = Some rD ->
+        exprD' tus tvs t e = Some eD ->
+        exists eD',
+          exprD' tus tvs t e' = Some eD' /\
+          forall us vs,
+            rD (eD us vs) (eD' us vs).
+    Hypothesis respectfulOk
+    : forall tus tvs e r rs t ts rD eD,
+        respectful e r = Some rs ->
+        RD r t = Some rD ->
+        exprD' tus tvs (fold_right (typ2 (F:=Fun)) t ts) e = Some eD ->
+        exists rD',
+          RD (fold_right Rrespects r rs) (fold_right (typ2 (F:=Fun)) t ts) = Some rD' /\
+          forall us vs,
+            Proper rD' (eD us vs).
+
+    Require Import MirrorCore.SubstI.
+    Lemma exprD'_App
+    : forall tus tvs td tr f x fD xD,
+        exprD' tus tvs (typ2 (F:=Fun) td tr) f = Some fD ->
+        exprD' tus tvs td x = Some xD ->
+        exprD' tus tvs tr (App f x) = Some (exprT_App fD xD).
+    Proof.
+      clear - Typ2Ok_Fun RSymOk_func RTypeOk_typD.
+      intros.
+      autorewrite with exprD_rw; simpl.
+      erewrite exprD_typeof_Some by eauto.
+      rewrite H. rewrite H0. reflexivity.
+    Qed.
+    Fixpoint apply_fold tus tvs t ts
+             (es : HList.hlist (fun t => ExprI.exprT tus tvs (typD t)) ts)
+    : ExprI.exprT tus tvs (typD (fold_right (typ2 (F:=Fun)) t ts))
+      -> ExprI.exprT tus tvs (typD t) :=
+      match es in HList.hlist _ ts
+            return ExprI.exprT tus tvs (typD (fold_right (typ2 (F:=Fun)) t ts))
+                   -> ExprI.exprT tus tvs (typD t)
+      with
+        | HList.Hnil => fun f => f
+        | HList.Hcons t' ts x xs => fun f =>
+                                      @apply_fold tus tvs t ts xs (exprT_App f x)
+      end.
+    Lemma apps_exprD'_fold_type
+    : forall tus tvs es e t eD,
+        exprD' tus tvs t (apps e es) = Some eD ->
+        exists ts fD esD,
+          exprD' tus tvs (fold_right (typ2 (F:=Fun)) t ts) e = Some fD /\
+          hlist_build (fun t => ExprI.exprT tus tvs (typD t))
+                      (fun t e => exprD' tus tvs t e) ts es = Some esD /\
+          forall us vs,
+            eD us vs = @apply_fold _ _ _ _ esD fD us vs.
+    Proof.
+      clear - Typ2Ok_Fun RTypeOk_typD RSymOk_func.
+      intros.
+      rewrite exprD'_apps in H; eauto.
+      unfold apps_sem' in H. forward. clear H.
+      revert H0; revert H1; revert eD; revert t; revert e0; revert e.
+      revert t0.
+      induction es; simpl; intros.
+      { exists nil. exists eD. exists HList.Hnil.
+        simpl. split; eauto.
+        forward. destruct r. inv_all; subst. assumption. }
+      { arrow_case_any.
+        { clear H.
+          red in x1. subst.
+          simpl in H1. autorewrite with eq_rw in H1.
+          forward; inv_all; subst.
+          eapply IHes with (e := App e a) in H1; eauto.
+          { forward_reason.
+            assert (x0 = fold_right (typ2 (F:=Fun)) t x1).
+            { autorewrite with exprD_rw in H1; simpl in H1.
+              forward; inv_all; subst.
+              eapply exprD_typeof_Some in H0; eauto.
+              eapply exprD_typeof_Some in H4; eauto.
+              rewrite H0 in H4.
+              inv_all. assumption. }
+            { subst.
+              eexists (x :: x1). exists e0.
+              eexists. split; eauto.
+              split. simpl.
+              rewrite H2. rewrite H. reflexivity.
+              simpl. intros.
+              erewrite exprD'_App in H1; eauto.
+              inv_all; subst. eauto. } }
+          { erewrite exprD'_App; eauto.
+            unfold exprT_App. autorewrite with eq_rw.
+            reflexivity. } }
+        { inversion H1. } }
+    Qed.
+
+    Inductive Forall3 {T U V : Type} (P : T -> U -> V -> Prop)
+    : list T -> list U -> list V -> Prop :=
+    | Forall3_nil : Forall3 P nil nil nil
+    | Forall3_cons : forall t u v ts us vs,
+                       P t u v -> Forall3 P ts us vs ->
+                       Forall3 P (t :: ts) (u :: us) (v :: vs).
+
+    Theorem rw_map2_sound
+    : forall T U V (f : T -> U -> mrw V) (P : T -> U -> V -> Prop) ts us vs,
+        rw_map2 f ts us = Some vs ->
+        (forall a b c, f a b = rw_ret c -> P a b c) ->
+        Forall3 P ts us vs.
+    Proof. clear. intros. revert H. revert vs; revert us.
+           induction ts; destruct us; simpl in *;
+           try solve [ inversion 1 ]; intros.
+           { inversion H. constructor. }
+           { specialize (H0 a u).
+             destruct (f a u); [ simpl in H | inversion H ].
+             specialize (IHts us).
+             destruct (rw_map2 f ts us); inversion H.
+             constructor; eauto. }
+    Qed.
+
+    Fixpoint recursive_rewrite (f : expr typ func)
+             (es : list (expr typ func * (R -> mrw (expr typ func))))
+             (rs : list R)
+    : mrw (expr typ func) :=
+      match es , rs with
+        | nil , nil => rw_ret f
+        | e :: es , r :: rs =>
+          rw_bind ((snd e) r)
+                  (fun e' => recursive_rewrite (App f e') es rs)
+        | _ , _ => rw_fail
+      end.
+
+    Lemma rw_bind_assoc
+    : forall {T U V} (c : mrw T) (k : T -> mrw U) (k' : U -> mrw V),
+        rw_bind (rw_bind c k) k' =
+        rw_bind c (fun x => rw_bind (k x) k').
+    Proof. clear.
+           destruct c; simpl; intros; auto.
+    Qed.
+    Lemma Proper_rw_bind (T U : Type)
+    : Proper (@eq (mrw T) ==> (pointwise_relation T (@eq (mrw U))) ==> @eq (mrw U)) (@rw_bind T U).
+    Proof.
+      clear. compute. intros; subst.
+      destruct y; auto.
+    Qed.
+    Lemma rw_bind_rw_ret
+    : forall {T U} (x : T) (k : T -> mrw U),
+        rw_bind (rw_ret x) k = k x.
+    Proof. clear. reflexivity. Qed.
+
+    Theorem recursive_rewrite_is_map2
+    : forall f es rs,
+        recursive_rewrite f es rs =
+        rw_bind (rw_map2 (fun e r => snd e r) es rs)
+                (fun es' => rw_ret (apps f es')).
+    Proof.
+      clear.
+      intros f es; revert f.
+      induction es; destruct rs; simpl; intros; auto.
+      rewrite rw_bind_assoc.
+      eapply Proper_rw_bind; auto.
+      red; intros.
+      rewrite IHes.
+      rewrite rw_bind_assoc.
+      eapply Proper_rw_bind; auto.
+      red; intros.
+      rewrite rw_bind_rw_ret. reflexivity.
+    Qed.
+
+    Inductive Forall2_hlist2 {T U : Type} (F : U -> Type)
+              (P : T -> forall u : U,F u -> F u -> Prop)
+    : list T -> forall us : list U, HList.hlist F us -> HList.hlist F us -> Prop :=
+    | Forall2_hlist2_nil : Forall2_hlist2 P nil HList.Hnil HList.Hnil
+    | Forall2_hlist2_cons : forall t u x y ts us xs ys,
+                              P t u x y ->
+                              Forall2_hlist2 P ts xs ys ->
+                              @Forall2_hlist2 T U F P (t :: ts) (u :: us)
+                                              (HList.Hcons x xs)
+                                              (HList.Hcons y ys).
+
+    Require Import MirrorCore.Util.Forwardy.
+
+    Lemma rw_map2_for_rewrite_recursive
+    : forall es rs es',
+        rw_map2 (fun ef r => snd ef r) es rs = Some es' ->
+        forall tus tvs ts esD,
+          setoid_rewrite2_rec tus tvs es ->
+          Forall2 (fun t r => exists rD, RD r t = Some rD) ts rs ->
+          hlist_build (fun t => ExprI.exprT tus tvs (typD t))
+                      (fun t e => exprD' tus tvs t (fst e)) ts es = Some esD ->
+          exists esD',
+            hlist_build (fun t => ExprI.exprT tus tvs (typD t))
+                        (fun t e => exprD' tus tvs t e) ts es' = Some esD' /\
+            Forall2_hlist2 (fun r t (e e' : ExprI.exprT tus tvs (typD t)) =>
+                              forall us vs rD,
+                                RD r t = Some rD ->
+                                rD (e us vs) (e' us vs)) rs esD esD'.
+    Proof.
+      induction es; destruct ts; destruct rs; simpl in *; intros;
+      try solve [ inversion H | inversion H1 ].
+      { inversion H2; subst. inversion H.
+        eexists; split; eauto. constructor. }
+      { unfold rw_bind in H.
+        forwardy. inv_all; subst.
+        inversion H1; clear H1; subst.
+        inversion H0; clear H0; subst.
+        eapply IHes in H5; eauto.
+        forward_reason.
+        eapply H6 in H3; eauto.
+        forward_reason.
+        Cases.rewrite_all_goal.
+        eexists; split; eauto.
+        constructor; eauto.
+        { intros. rewrite H1 in *. inv_all. subst. eauto. } }
+    Qed.
+
+    Theorem recursive_rewrite_sound
+    : forall tus tvs t r rD',
+        RD r t = Some rD' ->
+        forall es f f' rs e',
+        recursive_rewrite f' es rs = rw_ret e' ->
+        forall ts fD rD eD fD'
+               (Hrws : setoid_rewrite2_rec tus tvs es),
+          exprD' tus tvs t (apps f (map fst es)) = Some eD ->
+          exprD' tus tvs (fold_right (typ2 (F:=Fun)) t ts) f = Some fD ->
+          exprD' tus tvs (fold_right (typ2 (F:=Fun)) t ts) f' = Some fD' ->
+          RD (fold_right Rrespects r rs) (fold_right (typ2 (F:=Fun)) t ts) = Some rD ->
+          exists eD',
+            exprD' tus tvs t e' = Some eD' /\
+            forall us vs,
+              rD (fD us vs) (fD' us vs) ->
+              rD' (eD us vs) (eD' us vs).
+    Proof.
+      clear reflexiveOk transitiveOk rwOk respectfulOk.
+      clear rw respectful reflexive transitive.
+      induction es; destruct rs; simpl in *.
+      { inversion 1; subst. clear H0.
+        intros.
+        match goal with
+          | H : RD _ ?t = _ , H' : RD _ ?t' = _ |- _ =>
+            let HH := fresh in
+            (assert (HH : t = t')); [ | destruct HH ]
+        end.
+        { (* [R] has at most 1 type *) admit. }
+        revert H0. revert H3.
+        Cases.rewrite_all_goal. intros; inv_all; subst.
+        eexists; split; eauto. }
+      { inversion 1. }
+      { inversion 1. }
+      { intros.
+        consider (snd a r0); simpl; intros.
+        { arrow_case_any.
+          unfold Relim in H4; autorewrite with eq_rw in H4.
+          forwardy; inv_all; subst.
+          destruct ts.
+          { (** False **)
+            simpl in *. red in x1. subst.
+            clear IHes. exfalso. clear H6.
+            revert H9 H. clear.
+            (* [R] has at most 1 type *)
+            admit. }
+          { simpl in x1. red in x1.
+            generalize dependent x1.
+            intro. generalize x1.
+            inv_all; subst; intros.
+            generalize H1.
+            rewrite exprD'_apps in H1; eauto.
+            unfold apps_sem' in H1.
+            forwardy.
+            generalize (exprD'_typeof_expr _ (or_introl H2)).
+            simpl in H1. intro.
+            rewrite H10 in H1. unfold type_of_apply in H1.
+            forwardy. simpl in H11.
+            rewrite typ2_match_zeta in H11; eauto.
+            autorewrite with eq_rw in H11. forwardy.
+            inv_all; subst.
+            autorewrite with exprD_rw in H7. simpl in H7.
+            revert H7. Cases.rewrite_all_goal.
+            destruct y4.
+            change_rewrite H2. intro.
+            forwardy. inv_all; subst.
+            intro. inversion Hrws; clear Hrws; subst.
+            specialize (H15 _ _ H7 _ _ _ H0 H4).
+            forward_reason.
+            eapply IHes in H5; [ | eauto | eauto | eauto using exprD'_App
+                                 | eauto using exprD'_App
+                                 | eauto ].
+            forward_reason.
+            eexists; split; eauto.
+            clear - H14 H15 RelDec_Correct_eq_typ.
+            intros us vs.
+            unfold relation.
+            autorewrite with eq_rw.
+            unfold exprT_App in *.
+            generalize dependent (typ2_cast x (fold_right (typ2 (F:=Fun)) t ts)).
+            revert x1. revert y2.
+            simpl in *.
+            intros.
+            rewrite (UIP_refl x1) in H; clear x1.
+            generalize dependent (typD (typ2 x (fold_right (typ2 (F:=Fun)) t ts))).
+            intros; subst.
+            eapply H15; clear H15.
+            eapply H. eauto. }
+          { inversion H4. } }
+        { inversion H5. } }
+    Qed.
 
     Definition bottom_up (e : expr typ func) (r : R) : option (expr typ func) :=
       setoid_rewrite2
         (fun e efs r =>
 	   let es := map fst efs in
            rw_orelse
-	     match respectful e es r with
+	     match respectful e r with
 	       | None => rw (apps e es) r
 	       | Some rs =>
-		 rw_bind (rw_map2 (fun f r => (snd f) r) efs rs)
-			 (fun es' => rw_ret (apps e es'))
+		 rw_bind (recursive_rewrite e efs rs)
+			 (fun e' =>
+                            if transitive r
+                            then rw_orelse (rw e' r) (rw_ret e')
+                            else rw_ret e')
 	     end
 	     (if reflexive r then rw_ret (apps e es) else rw_fail))
         e nil r.
-  End bottom_up.
 
-  Section top_down.
-    Context (reflexive transitive : R -> bool)
-            (rw : expr typ func -> R -> option (expr typ func))
-            (respectful : expr typ func -> list (expr typ func) -> R -> option (list R)).
 
+    Lemma rw_orelse_sound : forall {T} (a b c : mrw T),
+                              rw_orelse a b = c ->
+                              (exists x, a = Some x /\ c = Some x) \/
+                              (a = rw_fail /\ b = c).
+    Proof. clear. intros. destruct a; eauto. Qed.
+
+    Theorem bottom_up_sound
+    : forall e e' tus tvs t rg rD eD,
+        bottom_up e rg = Some e' ->
+        RD rg t = Some rD ->
+        exprD' tus tvs t e = Some eD ->
+        exists eD',
+          exprD' tus tvs t e' = Some eD' /\
+          forall us vs,
+            rD (eD us vs) (eD' us vs).
+    Proof.
+      unfold bottom_up. intros.
+      eapply setoid_rewrite2_sound in H; eauto; try solve [ constructor ].
+      intros.
+      eapply rw_orelse_sound in H2; destruct H2; forward_reason.
+      { inv_all; subst.
+        consider (respectful e0 rg0); intros.
+        { unfold rw_bind in H6.
+          forwardy.
+          generalize H4.
+          eapply apps_exprD'_fold_type in H4.
+          forward_reason.
+          intro.
+          eapply respectfulOk in H2; eauto.
+          forward_reason.
+          eapply recursive_rewrite_sound with (r := rg0) (rs := l) in H6;
+            eauto.
+          forward_reason.
+          cut (   (Transitive rD0 /\ rw y rg0 = Some x)
+                  \/ (x = y)).
+          { clear H7. destruct 1.
+            { destruct H7.
+              eapply rwOk in H13. 3: eauto.
+              2: eauto.
+              destruct H13 as [ ? [ ? ? ] ].
+              eexists; split; eauto.
+              intros. etransitivity. eapply H12.
+              eapply H11. eauto. }
+            { subst.
+              eexists; split; eauto.
+              intros. eapply H12; eauto. eapply H11. } }
+          { consider (transitive rg0); intros.
+            * destruct (rw y rg0).
+              + left.
+                eapply transitiveOk in H7; eauto.
+              + right. inversion H13. reflexivity.
+            * right. inversion H13. reflexivity. } }
+        { eapply rwOk in H6; eauto. } }
+      { clear H2.
+        consider (reflexive rg0); intros.
+        { eapply reflexiveOk in H2; eauto.
+          inversion H6.
+          eexists; split; eauto. }
+        { inversion H6. } }
+    Qed.
+
+(*
     Fixpoint top_down (f : nat) (e : expr typ func) (r : R) {struct f}
     : option (expr typ func) :=
       setoid_rewrite2
@@ -252,16 +619,17 @@ Section setoid.
                            end
                          else
                            rw_ret e'))
-             match respectful e es r with
+             match respectful e r with
 	       | None => if reflexive r then rw_ret (apps e es) else rw_fail
 	       | Some rs =>
 	         rw_orelse
-                   (rw_bind (rw_map2 (fun f r => (snd f) r) efs rs)
-		            (fun es' => rw_ret (apps e es')))
+                   (recursive_rewrite e efs rs)
+		            (fun e' => rw_ret (apps e es')))
                    (if reflexive r then rw_ret (apps e es) else rw_fail)
 	     end)
         e nil r.
-  End top_down.
+*)
+  End top_bottom.
 
 End setoid.
 
@@ -290,45 +658,4 @@ Definition my_respectfulness' (f : expr nat nat)
         | Some e => true
         | None => false
       end.
-*)
-
-
-(*
-  Variable typeof_Rbase : Rbase -> option typ.
-  Fixpoint typeof_R (r : R) : option typ :=
-    match r with
-      | Rinj r => typeof_Rbase r
-      | Rrespects l r =>
-        match typeof_R l , typeof_R r with
-          | Some lt , Some rt => Some (typ2 lt rt)
-          | _ , _ => None
-        end
-      | Rpointwise t r =>
-        match typeof_R r with
-          | Some rt => Some (typ2 t rt)
-          | None => None
-        end
-    end.
-
-  Variable RbaseD : forall r : Rbase, match typeof_Rbase r with
-                                        | None => unit
-                                        | Some t => relation (typD t)
-                                      end.
-  Fixpoint RD (r : R) : match typeof_R r with
-                          | None => unit
-                          | Some t => relation (typD t)
-                        end.
-  refine
-    match r as r
-          return match typeof_R r with
-                   | None => unit
-                   | Some t => relation (typD t)
-                 end
-    with
-      | Rinj r => RbaseD r
-      | Rrespects l r =>
-        
-      | Rpointwise t r => _
-    end.
-  simpl.
 *)
